example/Fir.Check.fst
@@ -21,7 +21,7 @@ let bibo2_body (n: pos) (signal: ints): units =
   check "bibo" (sofar (abs signal <=^ const n) => (abs (fir2 signal) <=^ const n *^ const 10))
 
 let bibo2 n: ints -> units =
-  let e = Check.exp_of_stream1 (bibo2_body n) in
+  let unfold e = Check.exp_of_stream1 (bibo2_body n) in
   assert (Check.system_induct_k1 e) by (T.norm_full ["Fir.Check"]);
   Check.stream_of_checked1 e
 
@@ -31,6 +31,6 @@ let bibo3_body (n: pos) (signal: ints): units =
   check "bibo" (sofar (abs signal <=^ const n) => (abs (fir3 signal) <=^ const n *^ const 10))
 
 let bibo3 n: ints -> units =
-  let e = Check.exp_of_stream1 (bibo3_body n) in
+  let unfold e = Check.exp_of_stream1 (bibo3_body n) in
   assert (Check.system_induct_k 2 e) by (T.norm_full ["Fir.Check"]);
   Check.stream_of_checked1 e
