make/include/base.mk
@@ -24,14 +24,14 @@ FSTAR_DEP_OPT     ?= $(FSTAR_INCLUDES) $(FSTAR_CACHE)
 FSTAR_EXTRA_OPT   ?=
 FSTAR_OPT		  ?= $(FSTAR_INCLUDES) $(FSTAR_PROOF_OPT) $(FSTAR_CACHE) $(FSTAR_EXTRA_OPT) $(FSTAR_MAYBE_LAX) $(FSTAR_HINTS)
 
-FSTAR_SRCS = $(wildcard $(addsuffix /*.fst,$(FSTAR_SRC_DIRS)) $(addsuffix /*.fsti,$(FSTAR_SRC_DIRS)))
-FSTAR_ALL_SRCS = $(wildcard $(addsuffix /*.fst,$(FSTAR_ALL_INC_DIRS)) $(addsuffix /*.fsti,$(FSTAR_ALL_INC_DIRS)))
+FSTAR_SRCS ?= $(wildcard $(addsuffix /*.fst,$(FSTAR_SRC_DIRS)) $(addsuffix /*.fsti,$(FSTAR_SRC_DIRS)))
+FSTAR_ALL_SRCS ?= $(wildcard $(addsuffix /*.fst,$(FSTAR_ALL_INC_DIRS)) $(addsuffix /*.fsti,$(FSTAR_ALL_INC_DIRS)))
 
 all: verify
 .PHONY: all
 
 
-%/deps.mk: $(FSTAR_SRCS)
+%/deps.mk: $(FSTAR_SRCS) Makefile $(ROOT_DIR)/make/include/base.mk
 	@echo "[$(COMPONENT)] Updating dependencies"
 	@mkdir -p $(dir $@)
 	$(Q) $(FSTAR_EXE) $(FSTAR_DEP_OPT) --dep full $(FSTAR_SRCS) -o $@
